theories/iris/rules/iris_rules.v
@@ -3,7 +3,6 @@ From iris.program_logic Require Import language.
 From iris.proofmode Require Import base tactics classes.
 From iris.base_logic Require Export gen_heap ghost_map proph_map.
 From iris.base_logic.lib Require Export fancy_updates.
-Require Export iris iris_locations iris_properties iris_atomicity stdpp_aux.
 Require Export iris_rules_structural
         iris_rules_pure
         iris_rules_control
@@ -11,4 +10,3 @@ Require Export iris_rules_structural
         iris_rules_calls
         iris_rules_trap
         iris_rules_bind.
-Require Export datatypes operations properties opsem.
