theories/iris/rules/iris_rules_bind.v
@@ -3,10 +3,8 @@ From iris.program_logic Require Import language.
 From iris.proofmode Require Import base tactics classes.
 From iris.base_logic Require Export gen_heap ghost_map proph_map.
 From iris.base_logic.lib Require Export fancy_updates.
-Require Export datatypes operations properties opsem iris_rules_control iris_properties.
-Require Export iris_wp_def stdpp_aux.
+Require Export iris_rules_control.
 
-Close Scope byte_scope.
 
 Section bind_rules.
   
