theories/iris/rules/iris_rules_pure.v
@@ -3,10 +3,8 @@ From iris.program_logic Require Import language.
 From iris.proofmode Require Import base tactics classes.
 From iris.base_logic Require Export gen_heap ghost_map proph_map.
 From iris.base_logic.lib Require Export fancy_updates.
-Require Export iris_locations iris_properties iris_atomicity iris_wp_def.
+Require Export iris_wp_def.
 
-
-Close Scope byte_scope.
 
 (* basic instructions with simple(pure) reductions *)
 Section iris_rules_pure.
