theories/iris/rules/proofmode.v
@@ -2,15 +2,12 @@ From mathcomp Require Import ssreflect eqtype seq ssrbool.
 From iris.program_logic Require Import language.
 From iris.proofmode Require Import base tactics classes.
 From iris.bi Require Export weakestpre.
-Require Import iris iris_locations iris_properties iris_atomicity stdpp_aux.
 Require Import iris_rules iris_example_helper.
-Require Import datatypes operations properties opsem.
 
 Set Implicit Arguments.
 Unset Strict Implicit.
 Unset Printing Implicit Defensive.
 
-Close Scope byte_scope.
 
 Lemma build_llfill_local n f llh es e l1 l2 :
   llfill llh e = es ->
